simrel_cert_nforwarding_icf_R lemma proof

Coq/src/SimRelCertStepLemma.v
@@ -60,6 +60,7 @@ Section SimRelCertStepLemma.
   Notation "'Srf' S" := S.(ES.rf) (at level 10).
   Notation "'Sco' S" := S.(ES.co) (at level 10).
   Notation "'Scf' S" := S.(ES.cf) (at level 10).
+  Notation "'Sicf' S" := S.(ES.icf) (at level 10).
 
   Notation "'Sjfe' S" := S.(ES.jfe) (at level 10).
   Notation "'Srfe' S" := S.(ES.rfe) (at level 10).
@@ -148,142 +149,6 @@ Section SimRelCertStepLemma.
 
   Notation "'certX' S" := (fun k => (X ∩₁ SNTid_ S (ktid S k)) ∪₁ (kE S k)) (at level 1, only parsing).
 
-    Definition forwarding S lbl lbl' k k' e e'
-             (st st' : thread_st (ktid S k)) :=
-    ⟪ LBL  : lbl  = Slab S e ⟫ /\
-    ⟪ LBL' : lbl' = option_map (Slab S) e' ⟫ /\
-    ⟪ Kk   : K S (k , existT _ _ st ) ⟫ /\
-    ⟪ Kk'  : K S (k', existT _ _ st') ⟫ /\
-    ⟪ ADJ  : ES.cont_adjacent S k k' e e'⟫ /\
-    ⟪ STEP : ilbl_step (ktid S k) (opt_to_list lbl' ++ [lbl]) st st' ⟫ /\  
-    ⟪ CertRF : e2a S □ Sjf S ⨾ ⦗eq e⦘ ⊆ cert_rf G sc TC' (ktid S k) ⟫.  
-
-  Lemma forwarding_seqn_e S lbl lbl' k k' e e'
-             (st st' st'': thread_st (ktid S k))
-             (SRCC : simrel_cert prog S G sc TC TC' X k st st'')
-             (FRWD : forwarding S lbl lbl' k k' e e' st st') :
-    ES.seqn S e = eindex st.
-  Proof. 
-    assert (ES.Wf S) as WF.
-    { apply SRCC. }
-    assert (simrel_cont (stable_prog_to_prog prog) S G TC X) 
-      as SRCONT.
-    { apply SRCC. }
-    unfold forwarding in FRWD. desc.
-    set (AA := ADJ).
-    unfold ES.cont_adjacent in AA. desc.
-    unfold ES.cont_sb_dom in kSBDOM.
-    destruct k eqn:Heq.
-    { erewrite continit; eauto.
-      unfold ES.seqn.
-      arewrite (dom_rel (Ssb S ∩ ES.same_tid S ⨾ ⦗eq e⦘) ≡₁ ∅).
-      2 : by erewrite countNatP_empty.
-      split; [|done].
-      rewrite seq_eqv_r.
-      intros x [y [[SB STID] EQy]].
-      red. subst y.
-      eapply ES.init_tid_K; eauto.
-      exists (existT _ _ st), k.
-      splits; [by subst k|]. 
-      subst k. erewrite <- ES.cont_adjacent_tid_e; eauto.
-      rewrite <- STID.
-      assert (SEinit S x) as INITx.
-      { apply kSBDOM. basic_solver 10. }
-      red in INITx. unfolder in INITx. desf. }
-    erewrite contseqn; eauto.
-    erewrite ES.seqn_immsb; eauto.
-    { red. 
-      erewrite ES.cont_adjacent_tid_e 
-        with (k := k) (e := e); eauto.
-      2 : eby subst k.
-      unfold ES.cont_thread. desf. }
-    red. splits.
-    { assert (dom_rel (Ssb S ⨾ ⦗eq e⦘) eid) as HH.
-      { apply kSBDOM. basic_solver 10. }
-      unfolder in HH. desf. } 
-    intros x SB SB'.
-    assert (dom_rel ((Ssb S)^? ⨾ ⦗eq eid⦘) x) as HH.
-    { apply kSBDOM. basic_solver 10. }
-    unfolder in HH. desf.
-    { eapply ES.sb_irr; eauto. }
-    eapply ES.sb_irr; eauto.
-    eapply ES.sb_trans; eauto.
-  Qed.
-
-  Lemma forwarding_seqn_e' S lbl lbl' k k' e e'
-        (st st' st'': thread_st (ktid S k))
-        (SRCC : simrel_cert prog S G sc TC TC' X k st st'')
-        (FRWD : forwarding S lbl lbl' k k' e (Some e') st st') :
-    ES.seqn S e' = 1 + eindex st.
-  Proof. 
-    assert (ES.Wf S) as WF.
-    { apply SRCC. }
-    assert (simrel_cont (stable_prog_to_prog prog) S G TC X) 
-      as SRCONT.
-    { apply SRCC. }
-    set (AA := FRWD).
-    unfold forwarding in AA. desc.
-    set (AA := ADJ).
-    unfold ES.cont_adjacent in AA. desc.
-    assert (immediate (ES.sb S) e e') as IMMSB.
-    { apply ES.rmwi; auto.
-      apply RMWe. basic_solver. }
-    erewrite ES.seqn_immsb 
-      with (x := e); eauto; try red; splits.
-    { erewrite forwarding_seqn_e; eauto. }
-    erewrite ES.cont_adjacent_tid_e; eauto. 
-    erewrite ES.cont_adjacent_tid_e'
-      with (k := k); eauto. 
-  Qed.
-
-  Lemma forwarding_e2a_e S lbl lbl' k k' e e'
-             (st st' st'': thread_st (ktid S k))
-             (SRCC : simrel_cert prog S G sc TC TC' X k st st'')
-             (FRWD : forwarding S lbl lbl' k k' e e' st st') :
-    e2a S e = ThreadEvent (ES.cont_thread S k) (eindex st).
-  Proof. 
-    assert (ES.Wf S) as WF.
-    { apply SRCC. }
-    assert (ES.cont_adjacent S k k' e e') as ADJ.
-    { apply FRWD. }
-    rewrite e2a_ninit; auto.
-    2 : eapply ES.cont_adjacent_ninit_e; eauto.
-    erewrite ES.cont_adjacent_tid_e; eauto.
-    erewrite forwarding_seqn_e; eauto.
-  Qed.
-
-  Lemma forwarding_e2a_e' S lbl lbl' k k' e e'
-        (st st' st'': thread_st (ktid S k))
-        (SRCC : simrel_cert prog S G sc TC TC' X k st st'')
-        (FRWD : forwarding S lbl lbl' k k' e (Some e') st st') :
-    e2a S e' = ThreadEvent (ES.cont_thread S k) (1 + eindex st).
-  Proof. 
-    assert (ES.Wf S) as WF.
-    { apply SRCC. }
-    assert (ES.cont_adjacent S k k' e (Some e')) as ADJ.
-    { apply FRWD. }
-    rewrite e2a_ninit; auto.
-    2 : eapply ES.cont_adjacent_ninit_e'; eauto.
-    erewrite ES.cont_adjacent_tid_e'; eauto.
-    erewrite forwarding_seqn_e'; eauto.
-  Qed.
-
-  Lemma simrel_cert_forwarding_ex_ktid_cov lbl lbl' k k' e e' S 
-        (st st' st'': (thread_st (ktid S k)))
-        (SRCC : simrel_cert prog S G sc TC TC' X k st st'') 
-        (FRWD : forwarding S lbl lbl' k k' e e' st st')         
-        (CST_REACHABLE : (lbl_step (ktid S k))＊ st' st'') :
-    X ∩₁ Stid_ S (ktid S k') ∩₁ e2a S ⋄₁ C ⊆₁ kE S k'. 
-  Proof. 
-    assert (ES.Wf S) as WF.
-    { apply SRCC. }
-    arewrite (ktid S k' = ktid S k).
-    { symmetry. apply FRWD. }
-    etransitivity; [apply SRCC|].
-    eapply ES.cont_adjacent_sb_dom_mon; eauto.
-    apply FRWD.
-  Qed.
-
   Lemma simrel_cert_step_ex_ktid_cov k k' e e' S S'
         (st st' st'': (thread_st (ktid S k)))
         (SRCC : simrel_cert prog S G sc TC TC' X k st st'') 
@@ -309,41 +174,6 @@ Section SimRelCertStepLemma.
     basic_solver. 
   Qed.
   
-  Lemma simrel_cert_forwarding_cov_in_ex lbl lbl' k k' e e' S 
-        (st st' st'': (thread_st (ktid S k)))
-        (SRCC : simrel_cert prog S G sc TC TC' X k st st'') 
-        (FRWD : forwarding S lbl lbl' k k' e e' st st')         
-        (CST_REACHABLE : (lbl_step (ktid S k))＊ st' st'') :
-    e2a S ⋄₁ C ∩₁ kE S k' ⊆₁ X.
-  Proof. 
-    assert (ES.Wf S) as WF.
-    { apply SRCC. }
-    assert (ES.cont_adjacent S k k' e e') as ADJ.
-    { apply FRWD. }
-    rewrite ES.cont_adjacent_sb_dom 
-      with (k' := k'); eauto.
-    rewrite set_unionA.
-    rewrite set_inter_union_r.
-    unionL.
-    { rewrite set_interC. 
-      rewrite set_interC. 
-      apply SRCC. }
-    rewrite set_inter_union_r. 
-    unfolder. unionL.
-    { intros x [Cx EQx]. subst x. exfalso. 
-      eapply e2a_ge_ncov; eauto.
-      { apply FRWD. }
-      { erewrite ES.cont_adjacent_tid_e; eauto. }
-      erewrite forwarding_seqn_e; eauto. }
-    intros x [Cx EQx].
-    destruct e' as [e'|]; [|done].
-    subst x. exfalso. 
-    eapply e2a_ge_ncov; eauto.
-    { eapply ES.cont_adjacent_ninit_e'; eauto. }
-    { erewrite ES.cont_adjacent_tid_e'; eauto. }
-    erewrite forwarding_seqn_e'; eauto. 
-  Qed.
-
   Lemma simrel_cert_step_cov_in_ex k k' e e' S S'
         (st st' st'': (thread_st (ktid S k)))
         (SRCC : simrel_cert prog S G sc TC TC' X k st st'') 
@@ -381,81 +211,6 @@ Section SimRelCertStepLemma.
     omega.
   Qed.
 
-  Lemma simrel_cert_forwarding_kE_lab lbl lbl' k k' e e' S 
-        (st st' st'': (thread_st (ktid S k)))
-        (SRCC : simrel_cert prog S G sc TC TC' X k st st'') 
-        (FRWD : forwarding S lbl lbl' k k' e e' st st')         
-        (CST_REACHABLE : (lbl_step (ktid S k))＊ st' st'') :
-    eq_dom (kE S k' \₁ SEinit S) (Slab S) (Execution.lab (ProgToExecution.G st'') ∘ e2a S).
-  Proof. 
-    assert (ES.Wf S) as WF.
-    { apply SRCC. }
-    assert (simrel_cont (stable_prog_to_prog prog) S G TC X) 
-      as SRCONT.
-    { apply SRCC. } 
-    assert (ES.cont_adjacent S k k' e e') as ADJ.
-    { apply FRWD. }
-    set (AA := FRWD).
-    cdes AA.
-    assert (ktid S k = ktid S k') as kEQTID.
-    { by apply ADJ. }
-    assert (wf_thread_state (ktid S k) st) as WFst.
-    { eapply contwf; eauto. }
-    assert (wf_thread_state (ktid S k) st') as WFst'.
-    { rewrite kEQTID. eapply contwf; eauto. by rewrite <- kEQTID. }
-    assert (Gtid (e2a S e) = ES.cont_thread S k) as GTIDe.
-    { erewrite e2a_ninit; [|apply ADJ].
-      unfold Events.tid.
-      erewrite ES.cont_adjacent_tid_e; eauto. }
-    rewrite ES.cont_adjacent_sb_dom 
-      with (k' := k'); eauto.
-    rewrite set_unionA.
-    rewrite !set_minus_union_l.
-    rewrite !eq_dom_union. splits.
-    { apply SRCC. }
-    { intros x [EQx _]. subst x.
-      unfold compose.
-      erewrite steps_preserve_lab; eauto.
-      { rewrite <- LBL.
-        erewrite forwarding_e2a_e; eauto.
-        eapply ilbl_step_eindex_lbl; eauto. }
-      { by rewrite GTIDe. }
-      { apply lbl_steps_in_steps. 
-          by rewrite GTIDe. }
-      erewrite forwarding_e2a_e; eauto.
-      eapply acts_clos; eauto.
-      eapply ilbl_step_eindex_lt.
-      apply STEP. }
-    intros x [EQx _]. 
-    unfold eq_opt in EQx. 
-    destruct e' as [e'|]; [|done]. 
-    assert (Gtid (e2a S e') = ES.cont_thread S k) as GTIDe'.
-    { erewrite e2a_ninit.
-      2 : eapply ES.cont_adjacent_ninit_e'; eauto.
-      unfold Events.tid.
-      erewrite ES.cont_adjacent_tid_e'; eauto. }
-    subst x. unfold compose.
-    erewrite steps_preserve_lab; eauto.
-    { unfold option_map in LBL'.
-      destruct lbl' as [lbl'|]; 
-        inversion LBL' as [HLBL'].
-      rewrite <- HLBL'.
-      erewrite forwarding_e2a_e'; eauto.
-      eapply ilbl_step_eindex_lbl'; eauto. }
-    { by rewrite GTIDe'. }
-    { apply lbl_steps_in_steps. 
-        by rewrite GTIDe'. }
-    erewrite forwarding_e2a_e'; eauto.
-    eapply acts_clos; eauto.
-    erewrite ilbl_step_eindex_shift
-      with (st' := st'); eauto.
-    unfold option_map in LBL'.
-    destruct lbl' as [lbl'|].
-    2 : inversion LBL'.
-    unfold opt_to_list, app, length.
-    omega. 
-  Qed.
-
   Lemma simrel_cert_step_kE_lab k k' e e' S S'
         (st st' st'': (thread_st (ktid S k)))
         (SRCC : simrel_cert prog S G sc TC TC' X k st st'')
@@ -484,37 +239,6 @@ Section SimRelCertStepLemma.
     unfolder. ins. desf.
     { eapply basic_step_e2a_lab_e with (S:=S); eauto; apply SRCC. }
     eapply basic_step_e2a_lab_e' with (S:=S); eauto; apply SRCC.
-  Qed.
-
-  Lemma simrel_cert_forwarding_jf_in_cert_rf lbl lbl' k k' e e' S 
-        (st st' st'': (thread_st (ktid S k)))
-        (SRCC : simrel_cert prog S G sc TC TC' X k st st'')
-        (FRWD : forwarding S lbl lbl' k k' e e' st st')         
-        (CST_REACHABLE : (lbl_step (ktid S k))＊ st' st'') :
-    e2a S □ (Sjf S ⨾ ⦗kE S k'⦘) ⊆ cert_rf G sc TC' (ktid S k').
-  Proof.
-    assert (ES.Wf S) as WF.
-    { apply SRCC. }
-    assert (simrel_cont (stable_prog_to_prog prog) S G TC X) 
-      as SRCONT.
-    { apply SRCC. } 
-    assert (ES.cont_adjacent S k k' e e') as ADJ.
-    { apply FRWD. }
-    arewrite (ktid S k' = ktid S k).
-    { symmetry. apply ADJ. }
-    erewrite ES.cont_adjacent_sb_dom; eauto.
-    rewrite !id_union, !seq_union_r, !collect_rel_union.
-    unionL; auto.
-    { apply SRCC. }
-    { apply FRWD. }
-    unfold eq_opt.
-    destruct e' as [e'|].
-    2 : basic_solver.
-    assert (ES.rmw S e e') as RMW.
-    { eapply ES.cont_adjacent_rmw; eauto. }
-    apply ES.rmwD in RMW; auto.
-    rewrite ES.jfD; auto.
-    generalize RMW. type_solver. 
   Qed.
 
   Lemma simrel_cert_step_jf_in_cert_rf k k' e e' S S'
@@ -562,161 +286,6 @@ Section SimRelCertStepLemma.
     all: unfold jf_delta.
     { basic_solver. }
     desf. simpls. desf. unfolder. ins. desf. omega.
-  Qed.
-
-  Lemma simrel_cert_forwarding_ex_cont_iss lbl lbl' k k' e e' S 
-        (st st' st'': (thread_st (ktid S k)))
-        (SRCC : simrel_cert prog S G sc TC TC' X k st st'')
-        (FRWD : forwarding S lbl lbl' k k' e e' st st')         
-        (CST_REACHABLE : (lbl_step (ktid S k))＊ st' st'') :
-    X ∩₁ e2a S ⋄₁ (acts_set st'.(ProgToExecution.G) ∩₁ I) ⊆₁ dom_rel (Sew S ⨾ ⦗ kE S k' ⦘).
-  Proof. 
-    assert (ES.Wf S) as WFS.
-    { apply SRCC. }
-    assert (Execution.t S X) as EXEC.
-    { apply SRCC. }
-    assert (simrel_cont (stable_prog_to_prog prog) S G TC X) 
-      as SRCONT.
-    { apply SRCC. }
-    assert (ES.cont_adjacent S k k' e e') as ADJ.
-    { apply FRWD. }
-    erewrite ES.cont_adjacent_sb_dom; eauto.
-    edestruct ilbl_step_acts_set as [a [a' HH]].
-    { eapply wf_cont_state; eauto. }
-    { eapply FRWD. }
-    destruct HH as [EQa [EQa' ACTS]].
-    red in EQa, EQa', ACTS. 
-    rewrite ACTS.
-    rewrite !set_inter_union_l, !set_map_union.
-    rewrite !set_inter_union_r, !id_union, 
-    !seq_union_r, !dom_union.
-    apply set_union_Proper;
-      [apply set_union_Proper|].
-    { apply SRCC. }
-    { intros x [Xx [EQx Ix]].
-      assert (x = e) as EQe.
-      { edestruct e2a_eq_in_cf
-          with (x := x) (y := e) as [EQ | CF]; eauto.
-        { eapply Execution.ex_inE; eauto. }
-        { eapply ES.cont_adjacent_ninit_e; eauto. }
-        { rewrite <- EQx.
-          erewrite forwarding_e2a_e; eauto. }
-        exfalso. 
-        admit. }
-      admit. }
-    admit. 
-  Admitted.
-
-  Lemma simrel_cert_lbl_step_nrwm_eindex k S
-        (st st' st'': (thread_st (ktid S k)))
-        (SRCC : simrel_cert prog S G sc TC TC' X k st st'')
-        (LBL_STEP : lbl_step (ktid S k) st st')
-        (CST_REACHABLE : (lbl_step (ktid S k))＊ st' st'') :
-    ~ (codom_rel Grmw) (ThreadEvent (ktid S k) st.(eindex)).
-  Proof. 
-    assert (Wf G) as WFG by apply SRCC.
-    assert (ES.Wf S) as WFS by apply SRCC.
-    assert (Execution.t S X) as EXEC by apply SRCC.
-    assert (simrel_cont (stable_prog_to_prog prog) S G TC X) 
-      as SRCONT.
-    { apply SRCC. }
-    
-    intros [x RMW].
-    assert (exists xindex,
-               ⟪ ILT : xindex < eindex st ⟫ /\
-               x = ThreadEvent (ES.cont_thread S k) xindex).
-    { destruct x; simpls.
-      { apply WFG.(rmw_from_non_init) in RMW.
-        destruct_seq_l RMW as AA. desf. }
-      apply WFG.(rmw_in_sb) in RMW.
-      destruct_seq RMW as [AA BB].
-      red in RMW. desf.
-      eauto. }
-    desf.
-
-    assert (wf_thread_state (ktid S k) st) as WTS.
-    { eapply wf_cont_state; eauto. }
-    assert ((ProgToExecution.step (ktid S k))＊ st st') as STEPS.
-    { destruct LBL_STEP.
-      apply inclusion_t_rt. 
-      eapply ilbl_step_in_steps; eauto. }
-    assert (wf_thread_state (ktid S k) st') as WTS'.
-    { eapply wf_thread_state_steps; eauto. }
-    assert ((ProgToExecution.step (ES.cont_thread S k))＊ st' st'')
-      as STEPS'.
-    { apply lbl_steps_in_steps; eauto. }
-    assert (wf_thread_state (ES.cont_thread S k) st'') as WTS''.
-    { eapply wf_thread_state_steps; eauto. }
-
-    eapply eindex_not_in_rmw 
-      with (thread := ktid S k)
-           (st := st) (st' := st'); eauto.
-    { eapply ktid_ninit; eauto. }
-    assert (eindex st < eindex st') as LTST.
-    { edestruct LBL_STEP.
-      eapply ilbl_step_eindex_lt; eauto. }
-    assert (eindex st' <= eindex st'') as LTST'.
-    { eapply eindex_steps_mon; eauto. }
-    assert (acts_set (ProgToExecution.G st')
-                     (ThreadEvent (ktid S k) xindex))
-      as XINDST'.
-    { red. apply acts_clos; auto. omega. }
-    exists (ThreadEvent (ES.cont_thread S k) xindex).
-    eapply steps_dont_add_rmw; eauto.
-    apply seq_eqv_l. split; auto.
-    eapply dcertRMW. 
-    { apply SRCC. }
-    apply seq_eqv_lr. splits; auto.
-    all: apply acts_clos; auto.
-    all: omega.
-  Qed.
-
-  Lemma simrel_cert_forwarding_rmw_cov_in_kE lbl lbl' k k' e e' S
-        (st st' st'': (thread_st (ktid S k)))
-        (SRCC : simrel_cert prog S G sc TC TC' X k st st'')
-        (FRWD : forwarding S lbl lbl' k k' e e' st st')         
-        (CST_REACHABLE : (lbl_step (ktid S k))＊ st' st'') :
-    Grmw ⨾ ⦗C' ∩₁ e2a S □₁ kE S k'⦘ ⊆ e2a S □ Srmw S ⨾ ⦗ kE S k' ⦘.
-  Proof. 
-    assert (Wf G) as WFG by apply SRCC.
-    assert (ES.Wf S) as WFS.
-    { apply SRCC. }
-    assert (Execution.t S X) as EXEC.
-    { apply SRCC. }
-    assert (simrel_cont (stable_prog_to_prog prog) S G TC X) 
-      as SRCONT.
-    { apply SRCC. }
-    assert (simrel_e2a S G sc) as SRE2A.
-    { apply SRCC. }
-    assert (ES.cont_adjacent S k k' e e') as ADJ.
-    { apply FRWD. }
-    erewrite ES.cont_adjacent_sb_dom; eauto.
-    rewrite !set_collect_union.
-    rewrite !set_inter_union_r.
-    rewrite !id_union.
-    rewrite !seq_union_r, !collect_rel_union.
-    repeat apply union_mori.
-    { apply SRCC. }
-    { rewrite !seq_eqv_r.
-      intros x y [RMW [Cy [y' [EQy' E2Ae]]]].
-      subst y y'. exfalso. 
-      erewrite forwarding_e2a_e with (S := S) in RMW; eauto.
-      eapply simrel_cert_lbl_step_nrwm_eindex; eauto.
-      { eexists. apply FRWD. }
-      basic_solver. }       
-    unfold eq_opt.
-    destruct e' as [e'|].
-    2 : basic_solver. 
-    rewrite !seq_eqv_r.
-    intros x y [RMW [Cy [y' [EQy' E2Ae]]]].
-    subst y y'. 
-    exists e, e'. splits; auto.
-    { eapply ES.cont_adjacent_rmw; eauto. }
-    eapply wf_rmw_invf; eauto.
-    eapply e2a_rmw with (S := S); eauto.
-    red. do 2 eexists.
-    splits; eauto.
-    eapply ES.cont_adjacent_rmw; eauto. 
   Qed.
 
   Lemma simrel_cert_step_rmw_cov_in_kE k k' e e' S S'
@@ -774,41 +343,6 @@ Section SimRelCertStepLemma.
     apply RMW'. right. red. 
     unfold eq_opt. basic_solver. 
   Qed.
-
-  Lemma simrel_cert_forwarding lbl lbl' k k' e e' S
-        (st st' st'': thread_st (ktid S k))
-        (SRCC : simrel_cert prog S G sc TC TC' X k st st'')
-        (FRWD : forwarding S lbl lbl' k k' e e' st st')         
-        (CST_REACHABLE : (lbl_step (ktid S k))＊ st' st'') :
-    simrel_cert prog S G sc TC TC' X k' st' st''.
-  Proof. 
-    set (HH := FRWD).
-    unfold forwarding in HH. desc.
-    assert (ktid S k = ktid S k') as kEQTID.
-    { by apply ADJ. }
-    
-    constructor; auto. 
-    all: try (by try rewrite <- kEQTID; apply SRCC).
-    (* cstate : simrel_cstate S k' st' st'' *)      
-    { constructor. 
-      { eapply cstate_stable, SRCC. }
-      { red. exists st'. splits; eauto.
-          by rewrite <- kEQTID. }
-        by rewrite <- kEQTID. }
-    (* ex_ktid_cov : X ∩₁ STid ktid' ∩₁ e2a ⋄₁ C ⊆₁ kE' *)
-    { eapply simrel_cert_forwarding_ex_ktid_cov; eauto. }
-    (* cov_in_ex : e2a ⋄₁ C ∩₁ kE' ⊆₁ X *)
-    { eapply simrel_cert_forwarding_cov_in_ex; eauto. }
-    (* kE_lab : eq_dom (kE' \₁ SEinit) Slab (certG.(lab) ∘ e2a) *)
-    { eapply simrel_cert_forwarding_kE_lab; eauto. }
-    (* jf_in_cert_rf : e2a □ (Sjf ⨾ ⦗kE'⦘) ⊆ cert_rf G sc TC' ktid' *)
-    { eapply simrel_cert_forwarding_jf_in_cert_rf; eauto. }
-    (* ex_cont_iss : X ∩₁ e2a ⋄₁ (contE' ∩₁ I) ⊆₁ dom_rel (Sew ⨾ ⦗ kE' ⦘) *)
-    { eapply simrel_cert_forwarding_ex_cont_iss; eauto. }
-    (* rmw_cov_in_kE : Grmw ⨾ ⦗C' ∩₁ e2a □₁ kE'⦘ ⊆ e2a □ Srmw ⨾ ⦗kE'⦘ *)
-    { eapply simrel_cert_forwarding_rmw_cov_in_kE; eauto. }
-    admit.
-  Admitted.
   
   Lemma simrel_cert_lbl_step k S
         (st st' st'': thread_st (ktid S k))
@@ -889,6 +423,58 @@ Section SimRelCertStepLemma.
       as CONTDOMEQ.
     { eapply basic_step_e2a_set_collect_eq_dom; eauto.
       eapply kE_inE; eauto. }
+
+    assert (dom_rel (Sicf S') ⊆₁ SR S') as ICF_R.
+    { erewrite basic_step_icf; eauto.
+      rewrite dom_union. unionL.
+      { arewrite (dom_rel (Sicf S) ⊆₁ SE S ∩₁ SR S).
+        { apply set_subset_inter_r. split.
+          { admit. }
+          eapply icf_R; apply SRCC. }
+        (* TODO: introduce lemma *)
+        intros x [Ex Rx].
+        unfold is_r.
+        erewrite basic_step_lab_eq_dom; eauto. }
+      unfold icf_delta.
+      destruct 
+        (classic (is_r (Slab S') e))
+        as [Re|nRe].
+      { rewrite csE, dom_union. unionL.
+        2 : basic_solver. 
+        rewrite dom_cross.
+        2 : { intros HH. eapply HH. edone. } 
+        admit. }
+      intros x [y HH].
+      exfalso. 
+      apply nFRWD.
+      edestruct cstate_cont
+        as [s [EQs KK]]; [apply SRCC|].
+      red in EQs, KK. subst s.
+      assert (exists z, ES.cont_icf_dom S k z) 
+        as [z kICFz].
+      { generalize HH. basic_solver. }
+      edestruct ES.cont_icf_dom_cont_adjacent 
+        with (S := S) (k := k) (y := z)
+        as [k'' [a [a' ADJ]]]; eauto.
+      exists k'', a, a'.
+      edestruct ES.K_adj 
+        with (S := S) (k := k) (k' := k'')
+        as [ll [ll' [EQll [EQll' LSTEP]]]]; eauto.
+      { admit. }
+      red in EQll, EQll', LSTEP.
+      assert (ll = l) as HLL.
+      { admit. } 
+      assert (ll' = l') as HLL'.
+      { admit. } 
+      constructor; splits; auto.
+      { congruence. }
+      { congruence. }
+      { admit. }
+      { by rewrite <- EQlbl. }
+      arewrite (eq a ⊆₁ set_compl (is_r (Slab S))).
+      2 : rewrite ES.jfD; auto; basic_solver.
+      intros x' EQx' Ra. subst x'. 
+      admit. }
 
     exists k', S'. splits.
     { eapply basic_step_cont_thread_k; eauto. }
