Coq/src/SimRelCertForwarding.v
@@ -1,0 +1,737 @@
+Require Import Program.Basics Omega.
+From hahn Require Import Hahn.
+From imm Require Import Events Execution
+     Traversal TraversalConfig SimTraversal SimTraversalProperties
+     Prog ProgToExecution ProgToExecutionProperties Receptiveness
+     imm_common imm_s imm_s_hb SimulationRel
+     CertExecution2 CertExecutionMain
+     SubExecution CombRelations AuxRel.
+Require Import AuxRel.
+Require Import AuxDef.
+Require Import EventStructure.
+Require Import Consistency.
+Require Import Execution.
+Require Import BasicStep.
+Require Import AddJF.
+Require Import AddEW.
+Require Import AddCO.
+Require Import Step.
+Require Import StepWf.
+Require Import LblStep.
+Require Import CertRf.
+Require Import CertGraph.
+Require Import EventToAction.
+Require Import ImmProperties.
+Require Import SimRelCont.
+Require Import SimRelEventToAction.
+Require Import SimRel.
+Require Import SimRelCert.
+Require Import SimRelCertBasicStep.
+Require Import SimRelCertStep.
+Require Import ProgES.
+
+Set Implicit Arguments.
+Local Open Scope program_scope.
+
+Section SimRelCertForwarding.
+
+  Variable prog : stable_prog_type.
+  Variable G : execution.
+  Variable sc : relation actid.
+  Variable TC : trav_config.
+  Variable TC' : trav_config.
+  Variable X : eventid -> Prop.
+
+  Notation "'SE' S" := S.(ES.acts_set) (at level 10).
+  Notation "'SEinit' S" := S.(ES.acts_init_set) (at level 10).
+  Notation "'SEninit' S" := S.(ES.acts_ninit_set) (at level 10).
+  Notation "'Stid' S" := (S.(ES.tid)) (at level 10).
+  Notation "'Slab' S" := S.(ES.lab) (at level 10).
+  Notation "'Sloc' S" := (Events.loc S.(ES.lab)) (at level 10).
+
+  Notation "'Ssb' S" := S.(ES.sb) (at level 10).
+  Notation "'Srmw' S" := S.(ES.rmw) (at level 10).
+  Notation "'Sew' S" := S.(ES.ew) (at level 10).
+  Notation "'Sjf' S" := S.(ES.jf) (at level 10).
+  Notation "'Srf' S" := S.(ES.rf) (at level 10).
+  Notation "'Sco' S" := S.(ES.co) (at level 10).
+  Notation "'Scf' S" := S.(ES.cf) (at level 10).
+  Notation "'Sicf' S" := S.(ES.icf) (at level 10).
+
+  Notation "'Sjfe' S" := S.(ES.jfe) (at level 10).
+  Notation "'Srfe' S" := S.(ES.rfe) (at level 10).
+  Notation "'Scoe' S" := S.(ES.coe) (at level 10).
+  Notation "'Sjfi' S" := S.(ES.jfi) (at level 10).
+  Notation "'Srfi' S" := S.(ES.rfi) (at level 10).
+  Notation "'Scoi' S" := S.(ES.coi) (at level 10).
+
+  Notation "'Scc' S" := S.(cc) (at level 10).
+  Notation "'Ssw' S" := S.(sw) (at level 10).
+  Notation "'Shb' S" := S.(hb) (at level 10).
+  Notation "'Secf' S" := (S.(Consistency.ecf)) (at level 10).
+  Notation "'Seco' S" := (Consistency.eco S Weakestmo) (at level 10).
+
+  Notation "'SR' S" := (fun a => is_true (is_r S.(ES.lab) a)) (at level 10).
+  Notation "'SW' S" := (fun a => is_true (is_w S.(ES.lab) a)) (at level 10).
+  Notation "'SF' S" := (fun a => is_true (is_f S.(ES.lab) a)) (at level 10).
+
+  Notation "'SPln' S" := (fun a => is_true (is_only_pln S.(ES.lab) a)) (at level 10).
+  Notation "'SRlx' S" := (fun a => is_true (is_rlx S.(ES.lab) a)) (at level 10).
+  Notation "'SRel' S" := (fun a => is_true (is_rel S.(ES.lab) a)) (at level 10).
+  Notation "'SAcq' S" := (fun a => is_true (is_acq S.(ES.lab) a)) (at level 10).
+  Notation "'SAcqrel' S" := (fun a => is_true (is_acqrel S.(ES.lab) a)) (at level 10).
+  Notation "'SSc' S" := (fun a => is_true (is_sc S.(ES.lab) a)) (at level 10).
+
+  Notation "'K' S" := (S.(ES.cont_set)) (at level 10).
+
+  Notation "'Stid_' S" := (fun t x => Stid S x = t) (at level 1).
+  Notation "'SNTid_' S" := (fun t x => Stid S x <> t) (at level 1).
+
+  Notation "'GE'" := G.(acts_set).
+  Notation "'GEinit'" := (is_init ∩₁ GE).
+  Notation "'GEninit'" := ((set_compl is_init) ∩₁ GE).
+
+  Notation "'Glab'" := (Execution.lab G).
+  Notation "'Gloc'" := (Events.loc (lab G)).
+  Notation "'Gtid'" := (Events.tid).
+
+  Notation "'GTid' t" := (fun x => Gtid x = t) (at level 1).
+  Notation "'GNTid' t" := (fun x => Gtid x <> t) (at level 1).
+
+  Notation "'GR'" := (fun a => is_true (is_r Glab a)).
+  Notation "'GW'" := (fun a => is_true (is_w Glab a)).
+  Notation "'GF'" := (fun a => is_true (is_f Glab a)).
+
+  Notation "'GRel'" := (fun a => is_true (is_rel Glab a)).
+  Notation "'GAcq'" := (fun a => is_true (is_acq Glab a)).
+
+  Notation "'Gsb'" := (Execution.sb G).
+  Notation "'Grmw'" := (Execution.rmw G).
+  Notation "'Grf'" := (Execution.rf G).
+  Notation "'Gco'" := (Execution.co G).
+
+  Notation "'Grs'" := (imm_s_hb.rs G).
+  Notation "'Grelease'" := (imm_s_hb.release G).
+  Notation "'Gsw'" := (imm_s_hb.sw G).
+  Notation "'Ghb'" := (imm_s_hb.hb G).
+
+  Notation "'Gfurr'" := (furr G sc).
+  Notation "'Gvf' t" := (vf G sc TC' t) (at level 10, only parsing).
+
+  Notation "'Geco'" := (Execution_eco.eco G).
+
+  Notation "'C'"  := (covered TC).
+  Notation "'I'"  := (issued TC).
+  Notation "'C''"  := (covered TC').
+  Notation "'I''"  := (issued TC').
+  
+  Notation "'thread_syntax' t"  := 
+    (Language.syntax (thread_lts t)) (at level 10, only parsing).  
+
+  Notation "'thread_st' t" := 
+    (Language.state (thread_lts t)) (at level 10, only parsing).
+
+  Notation "'thread_init_st' t" := 
+    (Language.init (thread_lts t)) (at level 10, only parsing).
+
+  Notation "'thread_cont_st' t" :=
+    (fun st => existT _ (thread_lts t) st) (at level 10, only parsing).
+
+  Notation "'cont_lang'" :=
+    (fun S k => thread_lts (ES.cont_thread S k)) (at level 10, only parsing).
+
+  Notation "'kE' S" := (fun k => ES.cont_sb_dom S k) (at level 1, only parsing).
+  Notation "'ktid' S" := (fun k => ES.cont_thread S k) (at level 1, only parsing).
+
+  Notation "'certX' S" := (fun k => (X ∩₁ SNTid_ S (ktid S k)) ∪₁ (kE S k)) (at level 1, only parsing).
+
+  Definition forwarding S lbl lbl' k k' e e'
+             (st st' : thread_st (ktid S k)) :=
+    ⟪ LBL  : lbl  = Slab S e ⟫ /\
+    ⟪ LBL' : lbl' = option_map (Slab S) e' ⟫ /\
+    ⟪ Kk   : K S (k , existT _ _ st ) ⟫ /\
+    ⟪ Kk'  : K S (k', existT _ _ st') ⟫ /\
+    ⟪ ADJ  : ES.cont_adjacent S k k' e e'⟫ /\
+    ⟪ STEP : ilbl_step (ktid S k) (opt_to_list lbl' ++ [lbl]) st st' ⟫ /\  
+    ⟪ CertRF : e2a S □ Sjf S ⨾ ⦗eq e⦘ ⊆ cert_rf G sc TC' (ktid S k) ⟫.  
+
+  Lemma forwarding_seqn_e S lbl lbl' k k' e e'
+        (st st' st'': thread_st (ktid S k))
+        (SRCC : simrel_cert prog S G sc TC TC' X k st st'')
+        (FRWD : forwarding S lbl lbl' k k' e e' st st') :
+    ES.seqn S e = eindex st.
+  Proof. 
+    assert (ES.Wf S) as WF.
+    { apply SRCC. }
+    assert (simrel_cont (stable_prog_to_prog prog) S G TC X) 
+      as SRCONT.
+    { apply SRCC. }
+    unfold forwarding in FRWD. desc.
+    set (AA := ADJ).
+    unfold ES.cont_adjacent in AA. desc.
+    unfold ES.cont_sb_dom in kSBDOM.
+    destruct k eqn:Heq.
+    { erewrite continit; eauto.
+      unfold ES.seqn.
+      arewrite (dom_rel (Ssb S ∩ ES.same_tid S ⨾ ⦗eq e⦘) ≡₁ ∅).
+      2 : by erewrite countNatP_empty.
+      split; [|done].
+      rewrite seq_eqv_r.
+      intros x [y [[SB STID] EQy]].
+      red. subst y.
+      eapply ES.init_tid_K; eauto.
+      exists (existT _ _ st), k.
+      splits; [by subst k|]. 
+      subst k. erewrite <- ES.cont_adjacent_tid_e; eauto.
+      rewrite <- STID.
+      assert (SEinit S x) as INITx.
+      { apply kSBDOM. basic_solver 10. }
+      red in INITx. unfolder in INITx. desf. }
+    erewrite contseqn; eauto.
+    erewrite ES.seqn_immsb; eauto.
+    { red. 
+      erewrite ES.cont_adjacent_tid_e 
+        with (k := k) (e := e); eauto.
+      2 : eby subst k.
+      unfold ES.cont_thread. desf. }
+    red. splits.
+    { assert (dom_rel (Ssb S ⨾ ⦗eq e⦘) eid) as HH.
+      { apply kSBDOM. basic_solver 10. }
+      unfolder in HH. desf. } 
+    intros x SB SB'.
+    assert (dom_rel ((Ssb S)^? ⨾ ⦗eq eid⦘) x) as HH.
+    { apply kSBDOM. basic_solver 10. }
+    unfolder in HH. desf.
+    { eapply ES.sb_irr; eauto. }
+    eapply ES.sb_irr; eauto.
+    eapply ES.sb_trans; eauto.
+  Qed.
+  
+  Lemma forwarding_seqn_e' S lbl lbl' k k' e e'
+        (st st' st'': thread_st (ktid S k))
+        (SRCC : simrel_cert prog S G sc TC TC' X k st st'')
+        (FRWD : forwarding S lbl lbl' k k' e (Some e') st st') :
+    ES.seqn S e' = 1 + eindex st.
+  Proof. 
+    assert (ES.Wf S) as WF.
+    { apply SRCC. }
+    assert (simrel_cont (stable_prog_to_prog prog) S G TC X) 
+      as SRCONT.
+    { apply SRCC. }
+    set (AA := FRWD).
+    unfold forwarding in AA. desc.
+    set (AA := ADJ).
+    unfold ES.cont_adjacent in AA. desc.
+    assert (immediate (ES.sb S) e e') as IMMSB.
+    { apply ES.rmwi; auto.
+      apply RMWe. basic_solver. }
+    erewrite ES.seqn_immsb 
+      with (x := e); eauto; try red; splits.
+    { erewrite forwarding_seqn_e; eauto. }
+    erewrite ES.cont_adjacent_tid_e; eauto. 
+    erewrite ES.cont_adjacent_tid_e'
+      with (k := k); eauto. 
+  Qed.
+
+  Lemma forwarding_e2a_e S lbl lbl' k k' e e'
+        (st st' st'': thread_st (ktid S k))
+        (SRCC : simrel_cert prog S G sc TC TC' X k st st'')
+        (FRWD : forwarding S lbl lbl' k k' e e' st st') :
+    e2a S e = ThreadEvent (ES.cont_thread S k) (eindex st).
+  Proof. 
+    assert (ES.Wf S) as WF.
+    { apply SRCC. }
+    assert (ES.cont_adjacent S k k' e e') as ADJ.
+    { apply FRWD. }
+    rewrite e2a_ninit; auto.
+    2 : eapply ES.cont_adjacent_ninit_e; eauto.
+    erewrite ES.cont_adjacent_tid_e; eauto.
+    erewrite forwarding_seqn_e; eauto.
+  Qed.
+
+  Lemma forwarding_e2a_e' S lbl lbl' k k' e e'
+        (st st' st'': thread_st (ktid S k))
+        (SRCC : simrel_cert prog S G sc TC TC' X k st st'')
+        (FRWD : forwarding S lbl lbl' k k' e (Some e') st st') :
+    e2a S e' = ThreadEvent (ES.cont_thread S k) (1 + eindex st).
+  Proof. 
+    assert (ES.Wf S) as WF.
+    { apply SRCC. }
+    assert (ES.cont_adjacent S k k' e (Some e')) as ADJ.
+    { apply FRWD. }
+    rewrite e2a_ninit; auto.
+    2 : eapply ES.cont_adjacent_ninit_e'; eauto.
+    erewrite ES.cont_adjacent_tid_e'; eauto.
+    erewrite forwarding_seqn_e'; eauto.
+  Qed.
+
+  Lemma simrel_cert_forwarding_ex_ktid_cov lbl lbl' k k' e e' S 
+        (st st' st'': (thread_st (ktid S k)))
+        (SRCC : simrel_cert prog S G sc TC TC' X k st st'') 
+        (FRWD : forwarding S lbl lbl' k k' e e' st st')         
+        (CST_REACHABLE : (lbl_step (ktid S k))＊ st' st'') :
+    X ∩₁ Stid_ S (ktid S k') ∩₁ e2a S ⋄₁ C ⊆₁ kE S k'. 
+  Proof. 
+    assert (ES.Wf S) as WF.
+    { apply SRCC. }
+    arewrite (ktid S k' = ktid S k).
+    { symmetry. apply FRWD. }
+    etransitivity; [apply SRCC|].
+    eapply ES.cont_adjacent_sb_dom_mon; eauto.
+    apply FRWD.
+  Qed.
+
+  Lemma simrel_cert_forwarding_cov_in_ex lbl lbl' k k' e e' S 
+        (st st' st'': (thread_st (ktid S k)))
+        (SRCC : simrel_cert prog S G sc TC TC' X k st st'') 
+        (FRWD : forwarding S lbl lbl' k k' e e' st st')         
+        (CST_REACHABLE : (lbl_step (ktid S k))＊ st' st'') :
+    e2a S ⋄₁ C ∩₁ kE S k' ⊆₁ X.
+  Proof. 
+    assert (ES.Wf S) as WF.
+    { apply SRCC. }
+    assert (ES.cont_adjacent S k k' e e') as ADJ.
+    { apply FRWD. }
+    rewrite ES.cont_adjacent_sb_dom 
+      with (k' := k'); eauto.
+    rewrite set_unionA.
+    rewrite set_inter_union_r.
+    unionL.
+    { rewrite set_interC. 
+      rewrite set_interC. 
+      apply SRCC. }
+    rewrite set_inter_union_r. 
+    unfolder. unionL.
+    { intros x [Cx EQx]. subst x. exfalso. 
+      eapply e2a_ge_ncov; eauto.
+      { apply FRWD. }
+      { erewrite ES.cont_adjacent_tid_e; eauto. }
+      erewrite forwarding_seqn_e; eauto. }
+    intros x [Cx EQx].
+    destruct e' as [e'|]; [|done].
+    subst x. exfalso. 
+    eapply e2a_ge_ncov; eauto.
+    { eapply ES.cont_adjacent_ninit_e'; eauto. }
+    { erewrite ES.cont_adjacent_tid_e'; eauto. }
+    erewrite forwarding_seqn_e'; eauto. 
+  Qed.
+
+  Lemma simrel_cert_forwarding_kE_lab lbl lbl' k k' e e' S 
+        (st st' st'': (thread_st (ktid S k)))
+        (SRCC : simrel_cert prog S G sc TC TC' X k st st'') 
+        (FRWD : forwarding S lbl lbl' k k' e e' st st')         
+        (CST_REACHABLE : (lbl_step (ktid S k))＊ st' st'') :
+    eq_dom (kE S k' \₁ SEinit S) (Slab S) (Execution.lab (ProgToExecution.G st'') ∘ e2a S).
+  Proof. 
+    assert (ES.Wf S) as WF.
+    { apply SRCC. }
+    assert (simrel_cont (stable_prog_to_prog prog) S G TC X) 
+      as SRCONT.
+    { apply SRCC. } 
+    assert (ES.cont_adjacent S k k' e e') as ADJ.
+    { apply FRWD. }
+    set (AA := FRWD).
+    cdes AA.
+    assert (ktid S k = ktid S k') as kEQTID.
+    { by apply ADJ. }
+    assert (wf_thread_state (ktid S k) st) as WFst.
+    { eapply contwf; eauto. }
+    assert (wf_thread_state (ktid S k) st') as WFst'.
+    { rewrite kEQTID. eapply contwf; eauto. by rewrite <- kEQTID. }
+    assert (Gtid (e2a S e) = ES.cont_thread S k) as GTIDe.
+    { erewrite e2a_ninit; [|apply ADJ].
+      unfold Events.tid.
+      erewrite ES.cont_adjacent_tid_e; eauto. }
+    rewrite ES.cont_adjacent_sb_dom 
+      with (k' := k'); eauto.
+    rewrite set_unionA.
+    rewrite !set_minus_union_l.
+    rewrite !eq_dom_union. splits.
+    { apply SRCC. }
+    { intros x [EQx _]. subst x.
+      unfold compose.
+      erewrite steps_preserve_lab; eauto.
+      { rewrite <- LBL.
+        erewrite forwarding_e2a_e; eauto.
+        eapply ilbl_step_eindex_lbl; eauto. }
+      { by rewrite GTIDe. }
+      { apply lbl_steps_in_steps. 
+          by rewrite GTIDe. }
+      erewrite forwarding_e2a_e; eauto.
+      eapply acts_clos; eauto.
+      eapply ilbl_step_eindex_lt.
+      apply STEP. }
+    intros x [EQx _]. 
+    unfold eq_opt in EQx. 
+    destruct e' as [e'|]; [|done]. 
+    assert (Gtid (e2a S e') = ES.cont_thread S k) as GTIDe'.
+    { erewrite e2a_ninit.
+      2 : eapply ES.cont_adjacent_ninit_e'; eauto.
+      unfold Events.tid.
+      erewrite ES.cont_adjacent_tid_e'; eauto. }
+    subst x. unfold compose.
+    erewrite steps_preserve_lab; eauto.
+    { unfold option_map in LBL'.
+      destruct lbl' as [lbl'|]; 
+        inversion LBL' as [HLBL'].
+      rewrite <- HLBL'.
+      erewrite forwarding_e2a_e'; eauto.
+      eapply ilbl_step_eindex_lbl'; eauto. }
+    { by rewrite GTIDe'. }
+    { apply lbl_steps_in_steps. 
+        by rewrite GTIDe'. }
+    erewrite forwarding_e2a_e'; eauto.
+    eapply acts_clos; eauto.
+    erewrite ilbl_step_eindex_shift
+      with (st' := st'); eauto.
+    unfold option_map in LBL'.
+    destruct lbl' as [lbl'|].
+    2 : inversion LBL'.
+    unfold opt_to_list, app, length.
+    omega. 
+  Qed.
+
+  Lemma simrel_cert_forwarding_jf_in_cert_rf lbl lbl' k k' e e' S 
+        (st st' st'': (thread_st (ktid S k)))
+        (SRCC : simrel_cert prog S G sc TC TC' X k st st'')
+        (FRWD : forwarding S lbl lbl' k k' e e' st st')         
+        (CST_REACHABLE : (lbl_step (ktid S k))＊ st' st'') :
+    e2a S □ (Sjf S ⨾ ⦗kE S k'⦘) ⊆ cert_rf G sc TC' (ktid S k').
+  Proof.
+    assert (ES.Wf S) as WF.
+    { apply SRCC. }
+    assert (simrel_cont (stable_prog_to_prog prog) S G TC X) 
+      as SRCONT.
+    { apply SRCC. } 
+    assert (ES.cont_adjacent S k k' e e') as ADJ.
+    { apply FRWD. }
+    arewrite (ktid S k' = ktid S k).
+    { symmetry. apply ADJ. }
+    erewrite ES.cont_adjacent_sb_dom; eauto.
+    rewrite !id_union, !seq_union_r, !collect_rel_union.
+    unionL; auto.
+    { apply SRCC. }
+    { apply FRWD. }
+    unfold eq_opt.
+    destruct e' as [e'|].
+    2 : basic_solver.
+    assert (ES.rmw S e e') as RMW.
+    { eapply ES.cont_adjacent_rmw; eauto. }
+    apply ES.rmwD in RMW; auto.
+    rewrite ES.jfD; auto.
+    generalize RMW. type_solver. 
+  Qed.
+
+  Lemma simrel_cert_forwarding_ex_cont_iss lbl lbl' k k' e e' S 
+        (st st' st'': (thread_st (ktid S k)))
+        (SRCC : simrel_cert prog S G sc TC TC' X k st st'')
+        (FRWD : forwarding S lbl lbl' k k' e e' st st')         
+        (CST_REACHABLE : (lbl_step (ktid S k))＊ st' st'') :
+    X ∩₁ e2a S ⋄₁ (acts_set st'.(ProgToExecution.G) ∩₁ I) ⊆₁ dom_rel (Sew S ⨾ ⦗ kE S k' ⦘).
+  Proof. 
+    assert (ES.Wf S) as WFS.
+    { apply SRCC. }
+    assert (Execution.t S X) as EXEC.
+    { apply SRCC. }
+    assert (simrel_cont (stable_prog_to_prog prog) S G TC X) 
+      as SRCONT.
+    { apply SRCC. }
+    assert (ES.cont_adjacent S k k' e e') as ADJ.
+    { apply FRWD. }
+    erewrite ES.cont_adjacent_sb_dom; eauto.
+    edestruct ilbl_step_acts_set as [a [a' HH]].
+    { eapply wf_cont_state; eauto. }
+    { eapply FRWD. }
+    destruct HH as [EQa [EQa' ACTS]].
+    red in EQa, EQa', ACTS. 
+    rewrite ACTS.
+    rewrite !set_inter_union_l, !set_map_union.
+    rewrite !set_inter_union_r, !id_union, 
+    !seq_union_r, !dom_union.
+    apply set_union_Proper;
+      [apply set_union_Proper|].
+    { apply SRCC. }
+    { intros x [Xx [EQx Ix]].
+      assert (x = e) as EQe.
+      { edestruct e2a_eq_in_cf
+          with (x := x) (y := e) as [EQ | CF]; eauto.
+        { eapply Execution.ex_inE; eauto. }
+        { eapply ES.cont_adjacent_ninit_e; eauto. }
+        { rewrite <- EQx.
+          erewrite forwarding_e2a_e; eauto. }
+        exfalso. 
+        admit. }
+      admit. }
+    admit. 
+  Admitted.
+
+  Lemma simrel_cert_lbl_step_nrwm_eindex k S
+        (st st' st'': (thread_st (ktid S k)))
+        (SRCC : simrel_cert prog S G sc TC TC' X k st st'')
+        (LBL_STEP : lbl_step (ktid S k) st st')
+        (CST_REACHABLE : (lbl_step (ktid S k))＊ st' st'') :
+    ~ (codom_rel Grmw) (ThreadEvent (ktid S k) st.(eindex)).
+  Proof. 
+    assert (Wf G) as WFG by apply SRCC.
+    assert (ES.Wf S) as WFS by apply SRCC.
+    assert (Execution.t S X) as EXEC by apply SRCC.
+    assert (simrel_cont (stable_prog_to_prog prog) S G TC X) 
+      as SRCONT.
+    { apply SRCC. }
+    
+    intros [x RMW].
+    assert (exists xindex,
+               ⟪ ILT : xindex < eindex st ⟫ /\
+               x = ThreadEvent (ES.cont_thread S k) xindex).
+    { destruct x; simpls.
+      { apply WFG.(rmw_from_non_init) in RMW.
+        destruct_seq_l RMW as AA. desf. }
+      apply WFG.(rmw_in_sb) in RMW.
+      destruct_seq RMW as [AA BB].
+      red in RMW. desf.
+      eauto. }
+    desf.
+
+    assert (wf_thread_state (ktid S k) st) as WTS.
+    { eapply wf_cont_state; eauto. }
+    assert ((ProgToExecution.step (ktid S k))＊ st st') as STEPS.
+    { destruct LBL_STEP.
+      apply inclusion_t_rt. 
+      eapply ilbl_step_in_steps; eauto. }
+    assert (wf_thread_state (ktid S k) st') as WTS'.
+    { eapply wf_thread_state_steps; eauto. }
+    assert ((ProgToExecution.step (ES.cont_thread S k))＊ st' st'')
+      as STEPS'.
+    { apply lbl_steps_in_steps; eauto. }
+    assert (wf_thread_state (ES.cont_thread S k) st'') as WTS''.
+    { eapply wf_thread_state_steps; eauto. }
+
+    eapply eindex_not_in_rmw 
+      with (thread := ktid S k)
+           (st := st) (st' := st'); eauto.
+    { eapply ktid_ninit; eauto. }
+    assert (eindex st < eindex st') as LTST.
+    { edestruct LBL_STEP.
+      eapply ilbl_step_eindex_lt; eauto. }
+    assert (eindex st' <= eindex st'') as LTST'.
+    { eapply eindex_steps_mon; eauto. }
+    assert (acts_set (ProgToExecution.G st')
+                     (ThreadEvent (ktid S k) xindex))
+      as XINDST'.
+    { red. apply acts_clos; auto. omega. }
+    exists (ThreadEvent (ES.cont_thread S k) xindex).
+    eapply steps_dont_add_rmw; eauto.
+    apply seq_eqv_l. split; auto.
+    eapply dcertRMW. 
+    { apply SRCC. }
+    apply seq_eqv_lr. splits; auto.
+    all: apply acts_clos; auto.
+    all: omega.
+  Qed.
+
+    Lemma simrel_cert_forwarding_rmw_cov_in_kE lbl lbl' k k' e e' S
+        (st st' st'': (thread_st (ktid S k)))
+        (SRCC : simrel_cert prog S G sc TC TC' X k st st'')
+        (FRWD : forwarding S lbl lbl' k k' e e' st st')         
+        (CST_REACHABLE : (lbl_step (ktid S k))＊ st' st'') :
+    Grmw ⨾ ⦗C' ∩₁ e2a S □₁ kE S k'⦘ ⊆ e2a S □ Srmw S ⨾ ⦗ kE S k' ⦘.
+  Proof. 
+    assert (Wf G) as WFG by apply SRCC.
+    assert (ES.Wf S) as WFS.
+    { apply SRCC. }
+    assert (Execution.t S X) as EXEC.
+    { apply SRCC. }
+    assert (simrel_cont (stable_prog_to_prog prog) S G TC X) 
+      as SRCONT.
+    { apply SRCC. }
+    assert (simrel_e2a S G sc) as SRE2A.
+    { apply SRCC. }
+    assert (ES.cont_adjacent S k k' e e') as ADJ.
+    { apply FRWD. }
+    erewrite ES.cont_adjacent_sb_dom; eauto.
+    rewrite !set_collect_union.
+    rewrite !set_inter_union_r.
+    rewrite !id_union.
+    rewrite !seq_union_r, !collect_rel_union.
+    repeat apply union_mori.
+    { apply SRCC. }
+    { rewrite !seq_eqv_r.
+      intros x y [RMW [Cy [y' [EQy' E2Ae]]]].
+      subst y y'. exfalso. 
+      erewrite forwarding_e2a_e with (S := S) in RMW; eauto.
+      eapply simrel_cert_lbl_step_nrwm_eindex; eauto.
+      { eexists. apply FRWD. }
+      basic_solver. }       
+    unfold eq_opt.
+    destruct e' as [e'|].
+    2 : basic_solver. 
+    rewrite !seq_eqv_r.
+    intros x y [RMW [Cy [y' [EQy' E2Ae]]]].
+    subst y y'. 
+    exists e, e'. splits; auto.
+    { eapply ES.cont_adjacent_rmw; eauto. }
+    eapply wf_rmw_invf; eauto.
+    eapply e2a_rmw with (S := S); eauto.
+    red. do 2 eexists.
+    splits; eauto.
+    eapply ES.cont_adjacent_rmw; eauto. 
+  Qed.
+
+  Lemma simrel_cert_forwarding lbl lbl' k k' e e' S
+        (st st' st'': thread_st (ktid S k))
+        (SRCC : simrel_cert prog S G sc TC TC' X k st st'')
+        (FRWD : forwarding S lbl lbl' k k' e e' st st')         
+        (CST_REACHABLE : (lbl_step (ktid S k))＊ st' st'') :
+    simrel_cert prog S G sc TC TC' X k' st' st''.
+  Proof. 
+    set (HH := FRWD).
+    unfold forwarding in HH. desc.
+    assert (ktid S k = ktid S k') as kEQTID.
+    { by apply ADJ. }
+    
+    constructor; auto. 
+    all: try (by try rewrite <- kEQTID; apply SRCC).
+    (* cstate : simrel_cstate S k' st' st'' *)      
+    { constructor. 
+      { eapply cstate_stable, SRCC. }
+      { red. exists st'. splits; eauto.
+          by rewrite <- kEQTID. }
+        by rewrite <- kEQTID. }
+    (* ex_ktid_cov : X ∩₁ STid ktid' ∩₁ e2a ⋄₁ C ⊆₁ kE' *)
+    { eapply simrel_cert_forwarding_ex_ktid_cov; eauto. }
+    (* cov_in_ex : e2a ⋄₁ C ∩₁ kE' ⊆₁ X *)
+    { eapply simrel_cert_forwarding_cov_in_ex; eauto. }
+    (* kE_lab : eq_dom (kE' \₁ SEinit) Slab (certG.(lab) ∘ e2a) *)
+    { eapply simrel_cert_forwarding_kE_lab; eauto. }
+    (* jf_in_cert_rf : e2a □ (Sjf ⨾ ⦗kE'⦘) ⊆ cert_rf G sc TC' ktid' *)
+    { eapply simrel_cert_forwarding_jf_in_cert_rf; eauto. }
+    (* ex_cont_iss : X ∩₁ e2a ⋄₁ (contE' ∩₁ I) ⊆₁ dom_rel (Sew ⨾ ⦗ kE' ⦘) *)
+    { eapply simrel_cert_forwarding_ex_cont_iss; eauto. }
+    (* rmw_cov_in_kE : Grmw ⨾ ⦗C' ∩₁ e2a □₁ kE'⦘ ⊆ e2a □ Srmw ⨾ ⦗kE'⦘ *)
+    { eapply simrel_cert_forwarding_rmw_cov_in_kE; eauto. }
+    admit.
+  Admitted.
+
+  Lemma simrel_cert_nforwarding_icf_R lbl lbl' k k' e e' S S'
+        (st st' st'': thread_st (ktid S k))
+        (LBL  : lbl  = Slab S' e ) 
+        (LBL' : lbl' = option_map (Slab S') e')
+        (SRCC : simrel_cert prog S G sc TC TC' X k st st'')
+        (CertSTEP : cert_step G sc TC TC' X k k' st st' e e' S S')
+        (nFRWD : ~ exists k' e e', forwarding S lbl lbl' k k' e e' st st') :
+    dom_rel (Sicf S') ⊆₁ SR S'.
+  Proof.
+    cdes CertSTEP. cdes BSTEP_.
+    assert (ES.Wf S) as WFS.
+    { apply SRCC. }
+    assert (basic_step e e' S S') as BSTEP.
+    { econstructor; eauto. }
+    assert (simrel_cont (stable_prog_to_prog prog) S G TC X) 
+      as SRCONT.
+    { apply SRCC. } 
+
+    (* some technicalities *)
+    assert (lbl0 = lbl) as EQl.
+    { rewrite LBL, LAB'.
+      rewrite updo_opt, upds; auto.
+      unfold opt_ext in *.
+      basic_solver. }
+    assert (lbl'0 = lbl') as EQl'.
+    { rewrite LBL', LAB'.
+      unfold option_map, opt_same_ctor in *.
+      destruct e' as [e'|].
+      { destruct lbl'0; [|done].
+        unfold upd_opt.
+        by rewrite upds. }
+      destruct lbl'0; done. }
+    subst lbl0 lbl'0.
+
+    erewrite basic_step_icf; eauto.
+    rewrite dom_union. unionL.
+    { arewrite (dom_rel (Sicf S) ⊆₁ SE S ∩₁ SR S).
+      { apply set_subset_inter_r. split.
+        { rewrite ES.icfE; auto. basic_solver. }
+        eapply icf_R; apply SRCC. }
+      (* TODO: introduce lemma *)
+      intros x [Ex Rx].
+      unfold is_r.
+      erewrite basic_step_lab_eq_dom; eauto. }
+
+    unfold icf_delta.
+    destruct 
+      (classic (is_r (Slab S') e))
+      as [Re|nRe].
+    { rewrite csE, dom_union. unionL.
+      2 : basic_solver. 
+      rewrite dom_cross.
+      2 : { intros HH. eapply HH. edone. }
+      intros x kICFx.
+      assert ((Slab S □₁ ES.cont_icf_dom S k) (Slab S x)) 
+        as HH.
+      { basic_solver. }
+      eapply basic_step_cont_icf_dom_same_lab_u2v 
+        in HH; eauto.
+      unfold is_r in *.
+      arewrite (Slab S' x = Slab S x).
+      { erewrite basic_step_lab_eq_dom; eauto.
+        eapply ES.cont_icf_domE; eauto. }
+      unfold same_label_u2v in HH.
+      destruct (Slab S' e); try done.
+      destruct (Slab S x); done. }
+    
+    intros x [y HH].
+    exfalso. 
+    apply nFRWD.
+    edestruct cstate_cont
+      as [s [EQs KK]]; [apply SRCC|].
+    red in EQs, KK. subst s.
+    assert (exists z, ES.cont_icf_dom S k z) 
+      as [z kICFz].
+    { generalize HH. basic_solver. }
+    edestruct ES.cont_icf_dom_cont_adjacent 
+      with (S := S) (k := k) (e := z)
+      as [k''' [z' ADJ]]; eauto.
+    exists k''', z, z'.
+    edestruct simrel_cont_adjacent_inK'
+      with (S := S) (k := k) (k' := k''')
+      as [st''' KK''']; eauto.
+    edestruct ES.K_adj 
+      with (S := S) (k := k) (k' := k''') (st' := st''')
+      as [ll [ll' [EQll [EQll' LSTEP]]]]; eauto.
+    red in EQll, EQll', LSTEP.
+
+    edestruct nR_ilbl_step 
+      as [EQl [EQl' EQl'']].
+    { apply STEP. }
+    { apply LSTEP. }
+    { unfold is_r, id in *. 
+      by rewrite LBL. }
+    red in EQl, EQl', EQl''.
+
+    assert (st' = st''') as EQst.
+    { eapply unique_nR_ilbl_istep.
+      { eapply STEP. }
+      { eapply LSTEP. }
+      unfold is_r, id in *. 
+      by rewrite LBL. }
+    subst st'''.
+
+    constructor; splits; auto.
+    { congruence. }
+    { congruence. }
+    arewrite (eq z ⊆₁ set_compl (is_r (Slab S))).
+    2 : rewrite ES.jfD; auto; basic_solver.
+    intros z'' EQz''. subst z''. 
+    assert ((Slab S □₁ ES.cont_icf_dom S k) (Slab S z)) 
+      as HA.
+    { basic_solver. }
+    eapply basic_step_cont_icf_dom_same_lab_u2v 
+      in HA; eauto.
+    intros Rz. apply nRe.
+    unfold is_r in *.
+    unfold same_label_u2v in HA.    
+    destruct (Slab S z); try done.
+    destruct (Slab S' e); done.
+  Qed.
+  
+End SimRelCertForwarding.
